\documentclass{article}
\usepackage{amssymb}
\usepackage{../sty/proof}
\usepackage{../sty/bcprules}

\title{A proof of Peirce's Law equivalent to Law of Excluded Middle}
\author{Pasberth}
\date{January 28, 2014}

\begin{document}

\maketitle

\tableofcontents

\section{Deduction}
\subsection{Shorthands}

\begin{itemize}
\item negation $\neg \alpha$ is a shorthand for $\alpha \rightarrow \bot$
\item equivalent $\alpha \rightleftarrows \beta$ is a shorthand for $(\alpha \rightarrow \beta) \land (\beta \rightarrow \alpha)$
\end{itemize}
\subsection{Rules of Inference}

First, I prepare the following rules of inference, for the proof.

\infrule[Arr-Intro]
{
  \Gamma, \alpha \vdash \beta
}
{
  \Gamma \vdash \alpha \rightarrow \beta
}

\infrule[Arr-Elim]
{
  \Gamma_1 \vdash \alpha \andalso \Gamma_2 \vdash \alpha \rightarrow \beta
}
{
  \Gamma_1, \Gamma_2 \vdash \beta
}

\infrule[Conj-Intro]
{
  \Gamma_1 \vdash \alpha \andalso \Gamma_2 \vdash \beta
}
{
  \Gamma_1, \Gamma_2 \vdash \alpha \land \beta
}

\infrule[Conj-Elim-L]
{
  \Gamma \vdash \alpha \land \beta
}
{
  \Gamma \vdash \alpha
}

\infrule[Conj-Elim-R]
{
  \Gamma \vdash \alpha \land \beta
}
{
  \Gamma \vdash \beta
}

\infrule[Disj-Intro-L]
{
  \Gamma \vdash \alpha
}
{
  \Gamma \vdash \alpha \lor \beta
}

\infrule[Disj-Intro-R]
{
  \Gamma \vdash \beta
}
{
  \Gamma \vdash \alpha \lor \beta
}

\infrule[Disj-Elim]
{
  \Gamma_1 \vdash \alpha \lor \beta \andalso \Gamma_2, \alpha \vdash \gamma \andalso \Gamma_3, \beta \vdash \gamma
}
{
  \Gamma_1, \Gamma_2, \Gamma_3 \vdash \gamma
}

\infrule[Neg-Intro]
{
  \Gamma, \alpha \vdash \bot
}
{
  \Gamma \vdash \neg \alpha
}

\infrule[Neg-Elim]
{
  \Gamma_1 \vdash \alpha \andalso \Gamma_2 \vdash \neg \alpha
}
{
  \Gamma_1, \Gamma_2 \vdash \bot
}

\infrule[Bot-Elim]
{
  \Gamma \vdash \bot
}
{
  \Gamma \vdash \alpha
}

\section{De Morgan's Laws}
\subsection{Conjunction of Negations}

{\it Lemma}. $$\vdash \neg \alpha \land \neg \beta \rightarrow \neg (\alpha \lor \beta)$$
{\it Proof}. \\
\infer
{
  \vdash \neg \alpha \land \neg \beta \rightarrow \neg (\alpha \lor \beta)
}
{
  \infer
  {
    \neg \alpha \land \neg \beta \vdash \neg (\alpha \lor \beta)
  }
  {
    \infer
    {
      \alpha \lor \beta, \neg \alpha \land \neg \beta \vdash \bot
    }
    {
      \alpha \lor \beta \vdash \alpha \lor \beta
      &
      \infer
      {
        \alpha, \neg \alpha \land \neg \beta \vdash \bot
      }
      {
        \alpha \vdash \alpha
        &
        \infer
        {
          \neg \alpha \land \neg \beta \vdash \neg \alpha
        }
        {
          \neg \alpha \land \neg \beta \vdash \neg \alpha \land \neg \beta
        }
      }
      &
      \infer
      {
        \beta, \neg \alpha \land \neg \beta \vdash \bot
      }
      {
        \beta \vdash \beta
        &
        \infer
        {
          \neg \alpha \land \neg \beta \vdash \neg \beta
        }
        {
          \neg \alpha \land \neg \beta \vdash \neg \alpha \land \neg \beta
        }
      }
    }
  }
} \\
{\it Qed}. \\
\\
{\it Lemma}. $$\vdash \neg (\alpha \lor \beta) \rightarrow \neg \alpha \land \neg \beta$$
{\it Proof}. \\
\infer
{
  \vdash \neg (\alpha \lor \beta) \rightarrow \neg \alpha \land \neg \beta
}
{
  \infer
  {
    \neg (\alpha \lor \beta) \vdash \neg \alpha \land \neg \beta
  }
  {
    \infer
    {
      \neg (\alpha \lor \beta) \vdash \neg \alpha
    }
    {
      \infer
      {
        \alpha, \neg (\alpha \lor \beta) \vdash \bot
      }
      {
        \infer
        {
          \alpha \vdash \alpha \lor \beta
        }
        {
          \alpha \vdash \alpha
        }
        &
        \neg (\alpha \lor \beta) \vdash \neg (\alpha \lor \beta)
      }
    }
    &
    \infer
    {
      \neg (\alpha \lor \beta) \vdash \neg \beta
    }
    {
      \infer
      {
        \beta, \neg (\alpha \lor \beta) \vdash \bot
      }
      {
        \infer
        {
          \beta \vdash \alpha \lor \beta
        }
        {
          \beta \vdash \beta
        }
        &
        \neg (\alpha \lor \beta) \vdash \neg (\alpha \lor \beta)
      }
    }
  }
} \\
{\it Qed}. \\
\\
{\it Theorem}. $$\vdash \neg \alpha \land \neg \beta \rightleftarrows \neg (\alpha \lor \beta)$$
{\it Proof}. \\
\infer
{
  \vdash \neg \alpha \land \neg \beta \rightleftarrows \neg (\alpha \lor \beta)
}
{
  \infer
  {
    \vdash \neg \alpha \land \neg \beta \rightarrow \neg (\alpha \lor \beta)
  }
  {
    {\bf from\ above}
  }
  &
  \infer
  {
    \vdash \neg (\alpha \lor \beta) \rightarrow \vdash \neg \alpha \land \neg \beta
  }
  {
    {\bf from\ above}
  }
} \\
{\it Qed}.


\section{Peirce's Law equivalent to Law of Excluded Middle}

\subsection{Negation of Excluded Middle is False}

{\it Lemma}. $$\vdash \neg (\alpha \land \neg \alpha)$$
{\it Proof}. \\
\infer
{
  \vdash \neg (\alpha \land \neg \alpha)
}
{
  \infer
  {
    \alpha \land \neg \alpha \vdash \bot
  }
  {
    \infer
    {
      \alpha \land \neg \alpha \vdash \alpha
    }
    {
      \alpha \land \neg \alpha \vdash \alpha \land \neg \alpha
    }
    &
    \infer
    {
      \alpha \land \neg \alpha \vdash \neg \alpha
    }
    {
      \alpha \land \neg \alpha \vdash \alpha \land \neg \alpha
    }
  }
} \\
{\it Qed}. \\
\\
{\it Theorem}. $$\vdash \neg \neg (\alpha \lor \neg \alpha)$$
{\it Proof}. \\
\infer
{
  \vdash \neg \neg (\alpha \lor \neg \alpha)
}
{
  \infer
  {
    \neg (\alpha \lor \neg \alpha) \vdash \bot
  }
  {
    \infer
    {
      \vdash \neg (\neg \alpha \land \neg \neg \alpha)
    }
    {
      {\bf from\ above}
    }
    &
      \infer
      {
        \neg (\alpha \lor \neg \alpha) \vdash \neg \alpha \land \neg \neg \alpha
      }
      {
        \infer
        {
          \vdash \neg (\alpha \lor \neg \alpha) \rightarrow \neg \alpha \land \neg \neg \alpha
        }
        {
          {\bf De\ Morgen's\ Law}
        }
        &
        \neg (\alpha \lor \neg \alpha) \vdash \neg (\alpha \lor \neg \alpha)
      }
  }
} \\
{\it Qed}.

\subsection{Law of Excluded Middle implies Peirce's Law}

{\it Lemma}. $$\vdash \neg \alpha \lor \beta \rightarrow \alpha \rightarrow \beta$$
{\it Proof}. \\
\infer
{
  \vdash \neg \alpha \lor \beta \rightarrow \alpha \rightarrow \beta
}
{
  \infer
  {
    \neg \alpha \lor \beta \vdash \alpha \rightarrow \beta
  }
  {
    \neg \alpha \lor \beta \vdash \neg \alpha \lor \beta
    &
    \infer
    {
      \neg \alpha \vdash \alpha \rightarrow \beta
    }
    {
      \infer
      {
        \alpha, \neg \alpha \vdash \beta
      }
      {
        \infer
        {
          \alpha, \neg \alpha \vdash \bot
        }
        {
          \alpha \vdash \alpha
          &
          \neg \alpha \vdash \neg \alpha
        }
      }
    }
    &
    \infer
    {
      \beta \vdash \alpha \rightarrow \beta
    }
    {
      \alpha \vdash \alpha
      &
      \beta \vdash \beta
    }
  }
} \\
{\it Qed}. \\
\\
{\it Lemma}. $$\vdash \alpha \rightarrow \beta \rightarrow \alpha$$
{\it Proof}. \\
\infer
{
  \vdash \alpha \rightarrow \beta \rightarrow \alpha
}
{
  \infer
  {
    \alpha \vdash \beta \rightarrow \alpha
  }
  {
    \vdash \neg \beta \lor \alpha \rightarrow \beta \rightarrow \alpha
    &
    \infer
    {
      \alpha \vdash \neg \beta \lor \alpha
    }
    {
      \alpha \vdash \alpha
    }
  }
} \\
{\it Qed}. \\
\\
{\it Lemma}. $$\vdash \neg \alpha \rightarrow \alpha \rightarrow \beta$$
{\it Proof}. \\
\infer
{
  \vdash \neg \alpha \rightarrow \alpha \rightarrow \beta
}
{
  \infer
  {
    \neg \alpha \vdash \alpha \rightarrow \beta
  }
  {
    \vdash \neg \alpha \lor \beta \rightarrow \alpha \rightarrow \beta
    &
    \infer
    {
      \neg \alpha \vdash \neg \alpha \lor \beta
    }
    {
      \neg \alpha \vdash \neg \alpha
    }
  }
} \\
{\it Qed}. \\
\\

{\it Theorem}. $$(\alpha \lor \neg \alpha) \vdash ((\alpha \rightarrow \beta) \rightarrow \alpha) \rightarrow \alpha$$
{\it Proof}. \\
\infer
{
  \neg \alpha \vdash ((\alpha \rightarrow \beta) \rightarrow \alpha) \rightarrow \alpha
}
{
  \infer
  {
    \neg \alpha, (\alpha \rightarrow \beta) \rightarrow \alpha \vdash \alpha
  }
  {
    (\alpha \rightarrow \beta) \rightarrow \alpha \vdash (\alpha \rightarrow \beta) \rightarrow \alpha
    &
    \infer
    {
      \neg \alpha \vdash \alpha \rightarrow \beta
    }
    {
      \vdash \neg \alpha \rightarrow \alpha \rightarrow \beta
      &
      \neg \alpha \vdash \neg \alpha
    }
  }
} \\
\\
\infer
{
  \alpha \lor \neg \alpha \vdash ((\alpha \rightarrow \beta) \rightarrow \alpha) \rightarrow \alpha
}
{
  \alpha \lor \neg \alpha \vdash \alpha \lor \neg \alpha
  &
  \infer
  {
    \alpha \vdash ((\alpha \rightarrow \beta) \rightarrow \alpha) \rightarrow \alpha
  }
  {
    \vdash \alpha \rightarrow ((\alpha \rightarrow \beta) \rightarrow \alpha) \rightarrow \alpha
    &
    \alpha \vdash \alpha
  }
  &
  \infer
  {
    \neg \alpha \vdash ((\alpha \rightarrow \beta) \rightarrow \alpha) \rightarrow \alpha
  }
  {
    {\bf from\ above}
  }
} \\
{\it Qed}.

\subsection{Peirce's Law implies Law of Excluded Middle}

{\it Theorem}. $$\vdash \alpha \lor \neg \alpha$$
{\it Proof}. \\
\infer
{
  \vdash \alpha \lor \neg \alpha
}
{
  \infer
  {
    \vdash (((\alpha \lor \neg \alpha) \rightarrow \bot) \rightarrow \alpha \lor \neg \alpha) \rightarrow \alpha \lor \neg \alpha
  }
  {
    {\bf Peirce's\ Law}
  }
  &
  \infer
  {
    \vdash \neg (\alpha \lor \neg \alpha) \rightarrow \alpha \lor \neg \alpha
  }
  {
    \infer
    {
      \neg (\alpha \lor \neg \alpha) \vdash \alpha \lor \neg \alpha
    }
    {
      \infer
      {
        \neg (\alpha \lor \neg \alpha) \vdash \bot
      }
      {
        \neg (\alpha \lor \neg \alpha) \vdash \neg (\alpha \lor \neg \alpha)
        &
        \vdash \neg \neg (\alpha \lor \neg \alpha)
      }
    }
  }
} \\
{\it Qed}. \\

The proof ends here. Now, the law of excluded middle implies the Peirce's law and
the Peirce's law implies the law of excluded middle so both proofs are equivalent.

\end{document}