\documentclass{article}
\usepackage{sty/proof}
\pagestyle{empty}

\begin{document}

\section{P}

    \infer{
      \lambda x . f \left( x x \right)
      : \left( \left( \mu \tau_1 . \tau_1 \rightarrow \tau_2 \right) \rightarrow \tau_2 \right) \rightarrow \tau_2
    }{
    \infer{
      \lambda x . f \left( x x \right)
      : \left( \mu \tau_1 . \tau_1 \rightarrow \tau_2 \right) \rightarrow \tau_2
    }{
      \infer{
        f \left( x x \right)
        : \tau_2
      }{
        f : \tau_2 \rightarrow \tau_2
        &
        \infer{
          xx : \tau_2
        }{
          \infer{
            x : \left( \mu \tau_1 . \tau_1 \rightarrow \tau_2 \right) \rightarrow \tau_2
          }{
            x : \mu \tau_1 . \tau_1 \rightarrow \tau_2
          }
          &
          x : \mu \tau_1 . \tau_1 \rightarrow \tau_2
        }
      }
    }
    }

\section{Proof}

\infer{
  \lambda f .
  \left( \lambda x . f \left( x x \right) \right)
  \left( \lambda x . f \left( x x \right) \right)
  : \left( \tau_2 \rightarrow \tau_2 \right) \rightarrow \tau_2
}{
  \infer{
    \left( \lambda x . f \left( x x \right) \right)
    \left( \lambda x . f \left( x x \right) \right)
    : \tau_2
  }{
    {\large P}
    &
    \infer{
      \lambda x . f \left( x x \right)
      : \left( \mu \tau_1 . \tau_1 \rightarrow \tau_2 \right) \rightarrow \tau_2
    }{
      \infer{
        f \left( x x \right)
        : \tau_2
      }{
        f : \tau_2 \rightarrow \tau_2
        &
        \infer{
          xx : \tau_2
        }{
          \infer{
            x : \left( \mu \tau_1 . \tau_1 \rightarrow \tau_2 \right) \rightarrow \tau_2
          }{
            x : \mu \tau_1 . \tau_1 \rightarrow \tau_2
          }
          &
          x : \mu \tau_1 . \tau_1 \rightarrow \tau_2
        }
      }
    }
  }
}

\end{document}